\documentclass{ximera}

\input{../preamble.tex}

\author{Carl Stitz \and Jeff Zeager \and Bart Snapp \and Matthew Carr}
\license{CC-By-SA-NC}
\acknowledgement{http://www.stitz-zeager.com/}

\begin{document}
\begin{exercise}

\outcome{Work with exponential and logarithmic functions.}
\outcome{Know and use the properties of exponential and logarithmic functions.}

\tag{logarithms}




Use the properties of logarithms to write the expression as a single
logarithm. 

\begin{enumerate}
\item $4\ln(x) + 2\ln(y)\\=\answer{\ln(x^4y^2)}$ \label{combinelogfirst}
\item $\log_{2}(x) + \log_{2}(y) - \log_{2}(z)\\=\answer{\log_{2}(\frac{xy}{z})}$
\item $\log_{3}(x) - 2 \log_{3}(y)\\=\answer{\log_{3}(\frac{x}{y^2})}$
\item $\frac{1}{2}\log_{3}(x) - 2\log_{3}(y) - \log_{3}(z)\\=\answer{\log_{3}(\frac{\sqrt{x}}{y^2 z})}$
\item $2 \ln(x) -3 \ln(y) - 4\ln(z)\\=\answer{\ln(\frac{x^2}{y^3z^4})}$
\item $\ln(x) - \frac{1}{3} \ln(z) + \frac{1}{2} \ln(y)\\=\answer{\ln(\frac{x\sqrt{y}}{\sqrt[3]{z}})}$
\item $-\frac{1}{3} \ln(x) - \frac{1}{3}\ln(y) + \frac{1}{3} \ln(z)\\=\answer{\ln(\frac{1}{\sqrt[3]{xyz}})}$
\item $\log_{5}(x) - 3\\=\answer{\log_{5}(\frac{x}{125})}$
\item $\log_{7}(x) + \log_{7}(x - 3) - 2\\=\answer{\log_{7}(\frac{x(x-3)}{49}}$
\item $\ln(x) + \frac{1}{2}\\=\answer{\ln(\sqrt{e}x)}$ 
\item $\log_{2}(x) + \log_{4}(x)\\=\answer{\log_{4}(x^{3})}$ 
\item $\log_{2}(x) + \log_{4}(x-1)\\=\answer{\log_{4}(x^2(x-1))}$
\item $\log_{2}(x) + \log_{\frac{1}{2}}(x - 1)\\=\answer{\log_{2}(\frac{x}{x-1})}$ \label{combineloglast}
\end{enumerate}

\end{exercise}
\end{document}

